实现 sum(1)(2)(3) // 6

```js
function sum() {
  let args = [].slice.call(arguments);

  const temp = function() {
    let innerArgs = [].slice.call(arguments);
    args = args.concat(innerArgs);

    return sum.apply(null, args);
  };

  temp.valueOf = function() {
    return args.reduce(function(a, b, i) {
      return a + b;
    });
  };

  return temp.valueOf();
}
```

```js
function add() {
  var args = Array.prototype.slice.call(arguments);

  var fn = function() {
    var arg_fn = Array.prototype.slice.call(arguments);
    args = args.concat(arg_fn);
    console.log('fn', args);
    return add.apply(null, args);
  };

  fn.valueOf = function() {
    console.log('valueof', args);
    return args.reduce(function(a, b) {
      return a + b;
    });
  };

  return fn;
}
```

```js
var add = (...args) => {
  const temp = (...tempArgs) => {
    return add.apply(null, args.concat(tempArgs));
  }

  temp.valueOf = () => args.reduce((a, b) => a + b);

  return temp;
}
```

```js
[0, 1, 2, 3, 4].reduce(function(accumulator, currentValue, currentIndex, array) {
  console.log(accumulator, currentValue);
  return accumulator + currentValue;
});
```

```js
var add = a => {
  let sum = 0;
  sum += a;
  const temp = args => {
    console.log(args);
    if (!args) {
      return sum;
    } else {
      sum += args;
      return temp;
    }
  }

  return temp;
}
```
